src/util/bytes.dfy
@@ -23,4 +23,28 @@ module ByteHelpers {
     }
     return true;
   }
+
+  method Equal(bs1: Bytes, bs2: Bytes)
+    returns (eq: bool)
+    requires bs1.Valid() && bs2.Valid()
+    ensures eq == (bs1.data == bs2.data)
+  {
+    if bs1.Len() != bs2.Len() {
+      return false;
+    }
+    var i: uint64 := 0;
+    var len := bs1.Len();
+    while i < len
+      invariant i as nat <= |bs1.data|
+      invariant forall j:nat | j < i as nat :: bs1.data[j] == bs2.data[j]
+    {
+      var b1 := bs1.Get(i);
+      var b2 := bs2.Get(i);
+      if b1 != b2 {
+        return false;
+      }
+      i := i + 1;
+    }
+    return true;
+  }
 }
