src/util/lock_order.dfy
@@ -16,7 +16,7 @@ module LockOrder {
   // is it safe to acquire l, with locks held?
   function method safe_lock(locks: LockHint, l: uint64): bool
   {
-    locks == [] || l > locks[|locks|-1]
+    locks == [] || has_lock(locks, l) || l > locks[|locks|-1]
   }
 
   function method insert_lock_hint(locks: LockHint, h: uint64): LockHint
